feat: extend interval set

Regex/Interval.lean
@@ -1,5 +1,11 @@
 import Init.Data.Ord
+import Std.Data.Nat.Lemmas
+import Std.Data.Fin.Lemmas
+import Std.Data.Int.Lemmas
+import Std.Data.List.Basic
 import Regex.Utils
+import Regex.Bound
+import Regex.Data.Char.Basic
 
 /-!
 ## IntervalSet
@@ -8,56 +14,124 @@ This file contains an implementation of interval sets (`IntervalSet`),
 a sorted set of non-overlapping ranges (`Range`).
 -/
 
-class Bound (α : Type u) [Ord α] [LT α] where
-  min_value : α
-  max_value : α
-  as_u32 : α -> UInt32
-  increment : α -> α
-  decrement : α -> α
-
-instance : Bound Char where
-  min_value := '\u0000'
-  max_value := ⟨0x10FFFF, by simp_arith⟩
-  as_u32 (c : Char) := c.val
-  increment (c : Char) := if h : UInt32.isValidChar (c.val + 1) then ⟨c.val + 1, h⟩ else c
-  decrement (c : Char) := if h : UInt32.isValidChar (c.val - 1) then ⟨c.val - 1, h⟩ else c
-
-instance : HSub Char Char UInt32 where
-  hSub c₁ c₂ := c₁.val - c₂.val
-
 /-- A closed range bounded inclusively below and above (`start..end`). -/
-structure Range (α : Type u) [Ord α] [LT α] [Bound α] where
+structure Range (α : Type u) [Ord α] [LE α] [Bound α] where
   start: α
   «end»: α
+  isLe: start ≤ «end»
 deriving Repr, DecidableEq
+
+instance (α : Type u) [Ord α] [LE α] [LT α] [Bound α]: LT $ Range α where
+  lt r1 r2 := r1.end < r2.start
 
 instance : ToString $ Range Char where
   toString s := s!"{s.start} {s.end}"
 
-instance (α : Type u) [Ord α] [LT α] [Bound α] [Inhabited α] : Inhabited $ Range α where
-  default := ⟨default, default⟩
+instance : Inhabited $ Range Char where
+  default := ⟨default, default, of_decide_eq_true rfl⟩
 
 namespace Range
+
+/-- ranges `r1` and `r2` are non overlapping when they are sorted and
+    they are not overlapping or adjacent -/
+def nonOverlapping {α : Type u} [Ord α] [LE α] [LT α] [Bound α] [HSub α α Nat]
+    (r1 r2 : Range α) : Prop :=
+   1 < ((r2.start - r1.end) : Nat)
+
+instance {α : Type u} [Ord α] [LE α] [LT α] [Bound α] [HSub α α Nat]
+    (r1 r2 : Range α) : Decidable (Range.nonOverlapping r1 r2) :=
+  inferInstanceAs (Decidable (LT.lt 1 ((r2.start - r1.end) : Nat)))
 
 def intersection {α : Type u} [Ord α]
     [LT α] [LE α] [Bound α] [(a b : α) → Decidable (a ≤ b)]
     (r1 r2 : Range  α) : Option $ Range α :=
   let lower := if r1.start ≤ r2.start then r2.start else r1.start
   let upper := if r1.«end» ≤ r2.«end» then r1.«end» else r2.«end»
-  if lower ≤ upper then some ⟨lower, upper⟩
+  if h : lower ≤ upper then some ⟨lower, upper, h⟩
   else none
+
+instance : HSub Char Char Nat where
+  hSub c₁ c₂ := c₁.toNat - c₂.toNat
+
+def negate (r1 r2 : Range Char) (h : nonOverlapping r1 r2) : Range Char :=
+  ⟨Bound.increment r1.end, Bound.decrement r2.start, by
+    unfold nonOverlapping at h
+    unfold Bound.increment
+    unfold Bound.decrement
+    unfold instBoundCharInstOrdCharInstLEChar
+    simp_all
+    have h : 1 + r1.end.toNat < r2.start.toNat := by simp [Nat.add_lt_of_lt_sub h]
+    simp [Bound.Char.incr_le_decr h]⟩
 
 end Range
 
+namespace Ranges
+
+def unique (ranges: Array (Range Char)) : Array (Range Char) :=
+  match ranges.data with
+  | [] => #[]
+  | [r] => #[r]
+  | head :: tail  =>
+    let (_, unique) := tail |> List.foldl (init := (head, #[head]))
+      (fun (prev, unique) r =>
+        if prev = r then (r, unique)
+        else (r, unique.push r))
+    unique
+
+/-- an array of ranges is non overlapping when ranges are sorted
+    and no ranges are overlapping or adjacent -/
+def isNonOverlapping {α : Type u} [Ord α] [LT α] [LE α] [Bound α] [HSub α α Nat]
+    (ranges: Array (Range α)) : Prop :=
+  match ranges.data with
+  | [] => true
+  | [_] => true
+  | head :: tail  => List.Chain (Range.nonOverlapping) head tail
+
+theorem empty_isNonOverlapping {α : Type u} [Ord α] [LT α] [LE α] [Bound α] [HSub α α Nat]
+    : isNonOverlapping (#[] : Array (Range α)) := by
+  unfold isNonOverlapping
+  split <;> simp_all
+
+theorem single_isNonOverlapping (ranges : Array (Range Char)) (h : ranges.size = 1)
+    : isNonOverlapping ranges  := by
+  unfold isNonOverlapping
+  split <;> try simp_all
+  unfold Array.size at h
+  unfold List.length at h
+  split at h <;> try simp_all
+  unfold List.length at h
+  split at h <;> try simp_all
+
+theorem push_isNonOverlapping (ranges : Array (Range Char)) (r : Range Char)
+  (hp : ranges.pop? = some (last, rest))
+  (hr : isNonOverlapping ranges) (hlr : Range.nonOverlapping last r)
+    : isNonOverlapping (ranges.push r)  := by
+  sorry
+
+end Ranges
+
+theorem Array.size_one (a : α) : (#[a] : Array α).size = 1 := rfl
+
 /-- A sorted set of non-overlapping ranges. -/
-structure IntervalSet (α : Type u) [Ord α] [LT α] [Bound α] where
+structure IntervalSet (α : Type u) [Ord α] [LT α] [LE α] [Bound α] [HSub α α Nat]
+    [(a b : α) → Decidable (a < b)] [(a b : α) → Decidable (a = b)] where
   ranges: Array (Range α)
-deriving Repr, DecidableEq
+  isNonOverlapping: Ranges.isNonOverlapping ranges
+deriving Repr
 
 instance : ToString $ IntervalSet Char where
   toString s := s!"{s.ranges}"
 
+instance (α : Type u) [Ord α] [LT α] [LE α] [Bound α] [HSub α α Nat]
+    [(a b : α) → Decidable (a < b)] [(a b : α) → Decidable (a = b)]
+    : Inhabited $ IntervalSet α where
+  default := ⟨#[], Ranges.empty_isNonOverlapping⟩
+
 namespace Interval
+
+def singleton (r : Range Char) : IntervalSet Char :=
+  let arr := #[r]
+  ⟨arr, by simp [Ranges.single_isNonOverlapping arr (Array.size_one r)]⟩
 
 theorem pred_lt' {n m : Nat} (h : m < n) : Nat.pred n < n :=
   Nat.pred_lt (Nat.not_eq_zero_of_lt h)
@@ -69,70 +143,111 @@ def Fin.pred (i : Fin n) (h : 0 < i.val) : Fin n :=
     have h2 : i.val < n := i.isLt
     simp [Nat.lt_trans h1 h2]⟩
 
-/-- Converts this set into a canonical ordering. That is, every interval set contains an
-    ordered sequence of intervals where no two intervals are overlapping or adjacent. -/
-def canonicalize [Ord α] [HSub α α UInt32] [LT α] [Bound α] [ToString α]
-  [(a b : α) → Decidable (a < b)] [(a b : α) → Decidable (a = b)]
-    (interval : IntervalSet α) : IntervalSet α :=
-  let ranges := Array.qsort interval.ranges (fun a b => a.start < b.end)
+/-- Converts `ranges` into `IntervalSet` with canonical ordering.  -/
+def canonicalize (ranges : Array (Range Char)) : IntervalSet Char :=
+  let push (r : Range Char) (acc : IntervalSet Char) : IntervalSet Char :=
+    match hp : acc.ranges.pop? with
+    | some (last, rest) =>
+      if hr : Range.nonOverlapping last r then -- todo: prove it
+        let acc' := ⟨acc.ranges.push r,
+              Ranges.push_isNonOverlapping acc.ranges r hp acc.isNonOverlapping hr⟩
+        acc'
+      else panic s!"overlapping {last} {r}"
+    | none => singleton r
 
-  let init : Option (Range α) × Array (Range α) := (none, #[])
-  let (v, ranges) := ranges |> Array.foldl (init := init) (fun (v, acc) r =>
+  let _ranges := Array.qsort ranges
+                  (fun a b => a.start = b.start && a.end < b.end || a.start < b.start)
+  let _ranges := Ranges.unique _ranges
+
+  let init : Option (Range Char) × IntervalSet Char := (none, default)
+  let (v, intervalSet) := _ranges |> Array.foldl (init := init) (fun (v, acc) r =>
     match v with
     | some l =>
-      if (r.start - l.end).toNat = 1 then (some ⟨l.start, r.end⟩, acc) -- [a-bc-d] => [a-d]
-      else if r.start < l.end && l.start < r.start then (some ⟨l.start, r.end⟩, acc) -- [a-cb-d] => [a-d]
-      else if l.end < r.start then (r, acc.push l) -- [a-fg-h] => [a-fg-h]
-      else if l.end = r.start then (none, acc.push ⟨l.start, r.end⟩) -- [a-bb-c] => [a-c]
-      else if l.end < r.end then (none, acc.push r) -- [a-fb-c] => [a-f]
-      else (some r, acc.push l)
-    | none => (some r, acc))
+      if h : (r.start.val.toNat - l.end.val.toNat) = 1 then  -- [a-bc-d] => [a-d]
+          (some ⟨l.start, r.end, by
+            have hx : l.end < r.start := by simp [Char.succ_lt h]
+            have hy : l.end ≤ r.start := by simp [Char.lt_le hx]
+            have hz : l.start ≤ r.start := by simp [Char.le_trans l.isLe hy]
+            simp [Char.le_trans hz r.isLe]
+        ⟩, acc)
+      else if h: l.start = r.start then -- [a-ca-d] => [a-d]
+        if l.end < r.end
+        then (some ⟨l.start, r.end, by
+            have hx : l.start ≤ r.start := by simp [Char.eq_le h]
+            simp [Char.le_trans hx r.isLe]
+          ⟩, acc)
+        else (some l, acc) -- r.start = l.start ∧ r.end < l.end
+      else if r.start < l.end then -- [a-cb-d] => [a-d]
+        if r.end ≤ l.end -- [a-eb-d] => [a-e]
+        then (some l, acc)
+        else if h : l.start < r.start -- [a-cb-d] => [a-d]
+        then (some ⟨l.start, r.end, by
+            have hx : l.start ≤ r.start := by simp [Char.lt_le h]
+            simp [Char.le_trans hx r.isLe]
+          ⟩, acc)
+        else (some r, acc) -- r.start <= l.start ∧  l.end < r.end
+      else if l.end = r.start && r.start = r.end then (v, acc)
+      else if h : l.end = r.start then -- [a-bb-c] => [a-c]
+        let x : Range Char := ⟨l.start, r.end, by
+          have hx : l.end ≤ r.start := by simp [Char.eq_le h]
+          have hy : l.start ≤ r.start := by simp [Char.le_trans l.isLe hx]
+          simp [Char.le_trans hy r.isLe]
+        ⟩
+        (some x, acc)
+      else if r.start < l.start && l.end < r.end then (none, push r acc) -- [b-fa-g] => [a-g]
+      else if l.end.val + 1 < r.start.val then (r, push l acc) -- [a-eg-h] => [a-eg-h]
+      else (none, acc)
+    | none => (some r, default))
 
-  let ranges :=
+  let intervalSet :=
     match v with
-    | some v => ranges.push v
-    | none => ranges
+    | some v => push v intervalSet
+    | none => intervalSet
 
-  IntervalSet.mk (Array.qsort ranges (fun a b => a.start < b.end))
+  intervalSet
 
-/-- Negate a interval set with canonical ordering. -/
-def negate [Ord α] [LT α] [Bound α] [ToString α] [(a b : α) → Decidable (a < b)]
-    (interval : IntervalSet α) : IntervalSet α :=
+/-- Negate a interval set. -/
+def negate (interval : IntervalSet Char) : IntervalSet Char :=
   if interval.ranges.size = 0
-  then ⟨#[⟨Bound.min_value, Bound.max_value⟩]⟩
+  then
+    singleton ⟨(Bound.min_value : Char), Bound.max_value, Bound.min_value_le_max_value⟩
   else
-    let ranges : Array (Range α) :=
-      Array.mapIdx interval.ranges  (fun i x => (i,x))
+    let ranges : Array (Range Char) :=
+      Array.mapIdx interval.ranges  (fun i x => (i, x))
       |> Array.map (fun (i, y) =>
         if h : 0 < i.val
         then
           let j : Fin (Array.size interval.ranges) := Fin.pred i h
           let x := interval.ranges.get j
-          ⟨Bound.increment x.end, Bound.decrement y.start⟩
+          -- todo: prove it using nonOverlapping property
+          -- use Chain.chain_iff_get from mathlib
+          Range.negate x y (by sorry)
         else
           if Bound.min_value < y.start
-          then ⟨Bound.min_value, Bound.decrement y.start⟩
+          then ⟨Bound.min_value, Bound.decrement y.start, by
+              simp [Bound.min_value_le_decrement y.start]
+            ⟩
           else y
         )
-    let last :=
+    let last : Array (Range Char) :=
       match interval.ranges.pop? with
       | some (x, _) =>
           if x.end < Bound.max_value
-          then #[⟨Bound.increment x.end, Bound.max_value⟩]
+          then #[⟨Bound.increment x.end, Bound.max_value, by
+              simp [Bound.increment_le_max_value x.end]
+            ⟩]
           else #[]
       | none => #[]
-    ⟨ranges ++ last⟩
 
-/-- Intersection of interval sets with canonical ordering -/
-def intersection [Ord α] [LT α] [LE α] [Bound α] [ToString α] [Inhabited α]
-  [(a b : α) → Decidable (a ≤ b)] [(a b : α) → Decidable (a < b)]
-    (interval1 interval2 : IntervalSet α) : IntervalSet α :=
+    let ranges := ranges ++ last
+    canonicalize ranges
+
+/-- Intersection of interval sets -/
+def intersection (interval1 interval2 : IntervalSet Char) : IntervalSet Char :=
   let ranges := intersection.loop 0 0 interval1.ranges interval2.ranges #[]
-  ⟨ranges⟩
+  canonicalize ranges
 where
-  loop [Ord α] [LT α] [LE α][Bound α] [ToString α] [Inhabited α]
-    [(a b : α) → Decidable (a < b)] [(a b : α) → Decidable (a ≤ b)]
-    (a b : Nat) (ra rb acc : Array $ Range α) : Array $ Range α :=
+  loop (a b : Nat) (ra rb acc : Array $ Range Char) : Array $ Range Char :=
     if h₁ : a < ra.size then
       if h₂ : b < rb.size then
         let acc :=
@@ -147,23 +262,18 @@ where
     else acc
 termination_by _ a b ra rb _ => (ra.size - a, rb.size - b)
 
-/-- Subtract the interval set `interval2` from `interval1`, asumes canonical ordering. -/
-def difference [Ord α] [LT α] [LE α] [Bound α] [ToString α] [Inhabited α]
-  [(a b : α) → Decidable (a ≤ b)] [(a b : α) → Decidable (a < b)]
-    (interval1 interval2 : IntervalSet α) : IntervalSet α :=
+/-- Subtract the interval set `interval2` from `interval1`. -/
+def difference (interval1 interval2 : IntervalSet Char) : IntervalSet Char :=
   intersection interval1 (negate interval2)
 
-/-- Union of interval sets, result set has canonical ordering. -/
-def union [Ord α] [HSub α α UInt32] [LT α] [Bound α]
-    [ToString α] [(a b : α) → Decidable (a < b)] [(a b : α) → Decidable (a = b)]
-    (interval1 interval2 : IntervalSet α) : IntervalSet α :=
-  ⟨interval1.ranges ++ interval2.ranges⟩ |> canonicalize
+/-- Union of interval sets. -/
+def union (interval1 interval2 : IntervalSet Char) : IntervalSet Char :=
+  if interval1.ranges.size = 0 then interval2
+  else if interval2.ranges.size = 0 then interval1
+  else canonicalize (interval1.ranges ++ interval2.ranges)
 
-/-- Compute the symmetric difference (A⊖B = (A∪B)\(A∩B)) of the two sets,
-    asumes canonical ordering. -/
-def symmetric_difference [Ord α] [HSub α α UInt32] [LT α] [LE α] [Bound α] [ToString α] [Inhabited α]
-  [(a b : α) → Decidable (a ≤ b)] [(a b : α) → Decidable (a < b)] [(a b : α) → Decidable (a = b)]
-    (interval1 interval2 : IntervalSet α) : IntervalSet α :=
+/-- Compute the symmetric difference (A⊖B = (A∪B)\(A∩B)) of the two sets. -/
+def symmetric_difference (interval1 interval2 : IntervalSet Char) : IntervalSet Char :=
   let intervalI := intersection interval1 interval2
   let intervalU := union interval1 interval2
   difference intervalU intervalI
