Regex/Bound.lean
@@ -1,0 +1,172 @@
+import Init.Data.Ord
+import Std.Data.Nat.Lemmas
+import Std.Data.Fin.Lemmas
+import Std.Data.Int.Lemmas
+
+import Regex.Utils
+import Regex.Data.Fin.Basic
+import Regex.Data.Nat.Basic
+import Regex.Data.UInt.Basic
+import Regex.Data.Char.Basic
+
+/-!
+## Bound
+
+This file defines a `Bound` of type Char.
+A bound defines a bounded set of values with a min_value, max_value and increment
+and decrement operators. A `Range` is defined by a bound.
+-/
+
+namespace Bound
+
+theorem UInt32.isValidChar_lt_0x110000 (u : UInt32) (h : UInt32.isValidChar u)
+    : u.val.val < 0x110000 := by
+  unfold UInt32.isValidChar at h
+  unfold Nat.isValidChar at h
+  unfold UInt32.toNat at h
+  cases h
+  · rename_i h
+    have hy : u.val.val < 0x110000 := Nat.lt_trans h (by simp_arith)
+    simp_all [hy]
+  · rename_i h
+    simp_all [ h.right]
+
+theorem UInt32.isValidChar_lt_uintSize (u : UInt32) (h : UInt32.isValidChar u)
+    : u.val.val < UInt32.size := by
+  have hx : u.val.val < 0x110000 := UInt32.isValidChar_lt_0x110000 u h
+  have hy : u.val.val + 1 < 0x110000 + 1 := Nat.add_lt_add_right hx 1
+  have hz : 0x110000 + 1 < UInt32.size := by simp_arith
+  simp [Nat.lt_trans hy hz]
+
+theorem UInt32.isValidChar_succ_lt_uintSize (u : UInt32) (h : UInt32.isValidChar u)
+    : u.val.val + 1 < UInt32.size := by
+  have hx : u.val.val < 0x110000 := UInt32.isValidChar_lt_0x110000 u h
+  have hy : u.val.val + 1 < 0x110000 + 1 := Nat.add_lt_add_right hx 1
+  have hz : 0x110000 + 1 < UInt32.size := by simp_arith
+  simp [Nat.lt_trans hy hz]
+
+theorem UInt32.isValidChar_pred_lt_uintSize (u : UInt32) (h2 : UInt32.isValidChar u) (h3 : 1 ≤ u)
+    : u.val - 1 < UInt32.size := by
+
+  have hx1 : u.val.val < 0x110000 := UInt32.isValidChar_lt_0x110000 u h2
+  have hx2 : u.val < 0x110000 := UInt32.lt_def.mp hx1
+  have hx3 : 0x110000 < UInt32.size := by simp_arith
+  have hx4 : u.val < UInt32.size := Nat.lt_trans hx2 hx3
+
+  have h3 : u.val - 1 < UInt32.size := Nat.le_lt_sub_lt h3 hx4
+  simp [h3]
+
+theorem Nat.succ_lt_lt {c1 c2 : Nat} (h : 1 + c1 < c2) : c1 < c2 := by
+  have h1 : c1 < 1 + c1 := by
+    rw [Nat.add_comm]
+    simp[Nat.lt_succ_self _]
+  simp[Nat.lt_trans h1 h]
+
+theorem UInt32.lt_succ_le {c1 c2 : UInt32} (h : c1 < c2) (hsucc : c1.val + 1 < UInt32.size)
+    : c1 + 1 ≤ c2 := by
+  have hx : c1.val < c2.val := UInt32.lt_def.mp h
+  have heq : c1.val.val + 1 ≤ c2.val.val := Nat.succ_le_of_lt hx
+  have ht : c1.val.val + 1 = (c1 + 1).val.val := UInt32.toNat_add_toNat c1 1 hsucc
+  rw [ht] at heq
+  simp [UInt32.le_def.mpr heq]
+
+theorem UInt32.toNatUnfold (c1 c2 : UInt32) (heq : c2.toNat - c1.toNat = (c2 - c1).toNat)
+    : c2.val.val - c1.val.val = (c2 - c1).val.val := by
+  unfold UInt32.toNat at heq
+  simp_all [heq]
+
+theorem UInt32.lt_pred_le {c1 c2 : UInt32} (h : c1 < c2) (h2 : c2.val < UInt32.size)
+    : c1 ≤ c2 - 1  := by
+  have hx : c1.val < c2.val := UInt32.lt_def.mp h
+  have heq : c1.val.val ≤ c2.val.val - 1 := Nat.le_pred_of_lt hx
+  let hnm : 1 ≤ c2 := UInt32.one_le_of_lt h
+  have ht' : c2.toNat - 1 = (c2 - 1).toNat := UInt32.toNat_sub_toNat hnm h2
+  have ht : c2.val.val - 1 = (c2 - 1).val.val := UInt32.toNatUnfold 1 c2 ht'
+  rw [ht] at heq
+  simp [UInt32.le_def.mpr heq]
+
+theorem Char.succ_lt_lt {c1 c2 : Char} (h : 1 + Char.toNat c1 < Char.toNat c2) : c1 < c2 := by
+  have h : Char.toNat c1 < Char.toNat c2 := Nat.succ_lt_lt h
+  exact h
+
+theorem Char.succ_lt_succ_lt {c1 c2 : Char} (h : 1 + Char.toNat c1 < Char.toNat c2)
+    (hs: UInt32.isValidChar (c1.val + 1)) : ⟨c1.val + 1, hs⟩ < c2 := by
+  rw [Char.lt_def]
+  have h : c1.toNat + 1 < Char.toNat c2 := by
+    rw [Nat.add_comm]
+    simp [h]
+  have hx : Char.toNat c1 + 1 < UInt32.size := UInt32.isValidChar_succ_lt_uintSize c1.val c1.valid
+  have hy : c1.toNat + 1 = (c1.val + 1).toNat := UInt32.toNat_add_toNat c1.val 1 hx
+  rw [hy] at h
+  have hz : c1.val + 1 < c2.val := h
+  simp [hz]
+
+theorem Char.lt_pred_le {c1 c2 : Char} (h : c1 < c2) : c1.val ≤ c2.val - 1 := by
+  have h : c1.val < c2.val := Char.lt_def.mp h
+  have h2 : c2.val.val < UInt32.size := UInt32.isValidChar_lt_uintSize c2.val c2.valid
+  simp [UInt32.lt_pred_le h h2]
+
+theorem Char.lt_succ_le {c1 c2 : Char} (h : c1 < c2) : c1.val + 1 ≤ c2.val := by
+  have h : c1.val < c2.val := Char.lt_def.mp h
+  have hsucc : c1.val.val + 1 < UInt32.size := UInt32.isValidChar_succ_lt_uintSize c1.val c1.valid
+  simp [UInt32.lt_succ_le h hsucc]
+
+theorem Char.succ_add_le__pred {c1 c2 : Char} (h : 1 + c1.toNat < c2.toNat)
+  (hs: UInt32.isValidChar (c1.val + 1)) : c1.val + 1 ≤ c2.val - 1 := by
+  have h : ⟨c1.val + 1, hs⟩ < c2 := Char.succ_lt_succ_lt h hs
+  have h : c1.val + 1 ≤ c2.val - 1 := Char.lt_pred_le h
+  simp [h]
+
+theorem Char.incr_le_decr {c1 c2 : Char} (h : 1 + Char.toNat c1 < Char.toNat c2)
+    : Char.increment c1 ≤ Char.decrement c2 := by
+  unfold Char.increment
+  unfold Char.decrement
+  split <;> try simp_all
+  · split <;> try simp_all
+    · rename_i hs hp
+      let cs : Char := ⟨c1.val + 1, hs⟩
+      have hseq : cs = ⟨c1.val + 1, hs⟩ := by simp
+      let cp : Char := ⟨c2.val - 1, hp⟩
+      let hpeq : cp = ⟨c2.val - 1, hp⟩ := by simp
+      rw [← hseq, ← hpeq]
+      have h : cs.val ≤ cp.val := Char.succ_add_le__pred h hs
+      apply h
+    · rename_i hv _
+      have h : c1 < c2 := Char.succ_lt_lt h
+      have h : c1.val + 1 ≤ c2.val := by simp [Char.lt_succ_le h]
+      apply h
+  · split <;> try simp_all
+    · rename_i hv
+      have h : c1 < c2 := Char.succ_lt_lt h
+      have h : c1.val ≤ c2.val - 1 := by simp [Char.lt_pred_le h]
+      apply h
+    · have h : c1 < c2 := Char.succ_lt_lt h
+      simp [Char.lt_le h]
+
+end Bound
+
+/-- a Bound has a min_value, max_value and increment and decrement operators -/
+class Bound (α : Type u) [Ord α] [LE α] where
+  min_value : α
+  max_value : α
+  increment : α -> α
+  decrement : α -> α
+  min_value_le_max_value : min_value ≤ max_value
+  min_value_le_decrement c : min_value ≤ decrement c
+  increment_le_max_value c : increment c ≤ max_value
+
+/-- a Bound of type Char -/
+instance : Bound Char where
+  min_value := Char.min
+  max_value := Char.max
+  increment (c : Char) := Char.increment c
+  decrement (c : Char) := Char.decrement c
+  min_value_le_max_value := by simp_arith
+  increment_le_max_value c := by
+    unfold Char.increment; simp_all; split <;> try simp_all
+    · simp [Char.le_max]
+    · simp [Char.le_max]
+  min_value_le_decrement c := by
+    unfold Char.decrement; simp_all; split <;> try simp_all
+    · simp [Char.min_le]
+    · simp [Char.min_le]
