Regex/Data/Char/Basic.lean
@@ -1,0 +1,60 @@
+import Std.Data.Nat.Lemmas
+import Regex.Data.UInt.Basic
+
+namespace Char
+
+/-- max valid char -/
+def max : Char := ⟨0x10FFFF, by simp_arith⟩
+
+/-- incr char up to max valid char `Char.max` -/
+def increment (c : Char) : Char :=
+  if h : UInt32.isValidChar (c.val + 1) then ⟨c.val + 1, h⟩ else c
+
+/-- min valid char -/
+def min : Char := '\u0000'
+
+/-- decr char to min valid char `Char.min` -/
+def decrement (c : Char) : Char :=
+  if h : UInt32.isValidChar (c.val - 1) then ⟨c.val - 1, h⟩ else c
+
+theorem eq_le {c1 c2 : Char} (h : c1 = c2) : c1 ≤ c2 := by
+  have h₁ : c1.val.toNat ≤ c2.val.toNat := by simp[h]
+  exact h₁
+
+theorem lt_le {c1 c2 : Char} (h : c1 < c2) : c1 ≤ c2 := by
+  have h₁ : c1.val.toNat < c2.val.toNat := h
+  have h₂ : c1.val.toNat ≤ c2.val.toNat := by simp [Nat.le_of_lt h₁]
+  exact h₂
+
+theorem succ_lt {c1 c2 : Char} (h : (c2.val.toNat - c1.val.toNat) = 1) : c1 < c2 := by
+  have hx : c1.val.toNat < c2.val.toNat := by simp_all [Nat.lt_of_sub_eq_succ h]
+  exact hx
+
+theorem le_trans {c1 c2 c3 : Char} (h₁ : c1 ≤ c2) (h₂ : c2 ≤ c3) : c1 ≤ c3 := by
+  have h : c1.val.toNat ≤ c3.val.toNat := by exact Nat.le_trans h₁ h₂
+  exact h
+
+theorem min_le (c : Char) : Char.min ≤ c := by
+  have h : 0 ≤ c.val.toNat := by simp_all
+  exact h
+
+theorem le_max (c : Char) : c ≤ Char.max := by
+  cases c.valid
+  · rename_i h
+    have hx : 0xd800 < 0x10FFFF := by simp_arith
+    have hy : c.val.toNat < 0x10FFFF := by simp [Nat.lt_trans h hx]
+    have hz : c < Char.max := by exact hy
+    simp [Char.lt_le hz]
+  · rename_i h
+    have hx : c.val.toNat < 0x10FFFF.succ := h.right
+    have hy : c.val.toNat ≤ 0x10FFFF := Nat.le_of_lt_succ hx
+    exact hy
+
+theorem lt_def {a b : Char} : a < b ↔ a.val < b.val := .rfl
+
+theorem one_le_of_lt {c1 c2 : Char} (h : c1 < c2) : 1 ≤ c2.val :=
+  have h : c1.val < c2.val := Char.lt_def.mp h
+  UInt32.one_le_of_lt h
+
+theorem toNat_eq (c : Char) : c.val.toNat.toUInt32 = c.val := by
+  simp [UInt32.toNat_toUInt_eq c.val]
