Regex/Data/Fin/Basic.lean
@@ -1,0 +1,42 @@
+import Std.Data.Fin.Lemmas
+
+namespace Fin
+
+theorem ofNat_eq (n : Nat) (h : n < UInt32.size)
+    : (Fin.ofNat n : Fin UInt32.size) = ⟨n, h⟩  := by
+  have hu : UInt32.size = 4294967295 + 1 := by simp_arith
+  rw [hu] at h
+  unfold Fin.ofNat
+  simp [Fin.val_mk h]
+  simp_all [Nat.mod_eq_of_lt h]
+
+theorem ofNat_val_eq (n : Nat) (h : n < UInt32.size)
+    : (Fin.ofNat n : Fin UInt32.size).val = n := by
+  simp [Fin.ofNat_eq n h]
+
+theorem ofNat_add (n m : Nat) (h : n + m < UInt32.size)
+    : (Fin.ofNat (n + m) : Fin UInt32.size).val = n + m := by
+  have hu : UInt32.size = 4294967295 + 1 := by simp_arith
+  rw [hu] at h
+  unfold Fin.ofNat
+  simp [Fin.val_mk h]
+  simp_all [Nat.mod_eq_of_lt h]
+
+theorem toNat_ofNat_eq (n : Fin UInt32.size) : (Fin.ofNat (n.val)) = n := by
+  unfold Fin.ofNat
+  have heq : n.val % UInt32.size = n.val := by simp_all [Nat.mod_eq_of_lt n.isLt]
+  have hn : n.val % UInt32.size < UInt32.size := by rw[heq]; simp [n.isLt]
+  let m : Fin UInt32.size := { val := n.val % UInt32.size, isLt := hn }
+  have hm : m = { val := n.val % UInt32.size, isLt := hn } := by simp
+  rw [← hm]
+  simp [heq]
+
+theorem ofNat_val_add (n m : Fin UInt32.size) (h : n.val + m.val < UInt32.size)
+    : (Fin.ofNat (n.val + m.val)) = n + m := by
+  unfold Fin.ofNat
+  have heq : (n.val + m.val) % UInt32.size = n.val + m.val := by simp_all [Nat.mod_eq_of_lt h]
+  have hnm : (n.val + m.val) % UInt32.size < UInt32.size := by rw[heq]; simp [h]
+  let nm : Fin UInt32.size := { val := (n.val + m.val) % UInt32.size, isLt := hnm }
+  have hm : nm = { val := (n.val + m.val) % UInt32.size, isLt := hnm } := by simp
+  rw [← hm]
+  rw [Fin.add_def]
