Regex/Data/Nat/Basic.lean
@@ -1,0 +1,16 @@
+import Std.Data.Nat.Lemmas
+
+namespace Nat
+
+theorem mod_sub_eq_of_lt {i j n : Nat} (h : i ≤ j) (h1 : j - i < n) (h2 : i ≤ n)
+    : (j + (n - i)) % n = j - i := by
+  rw [← Nat.add_sub_assoc h2 j]
+  rw [Nat.sub_add_comm h]
+  have hy : ((j - i) + n) % n = (j - i) % n := Nat.add_mod_right (j - i) n
+  have h1 : (j - i) % n = j - i := Nat.mod_eq_of_lt h1
+  simp_all [hy]
+
+theorem le_lt_sub_lt {i j n : Nat} (h1 : i ≤ j) (h2 : j < n) :  j - i < n := by
+  have hy : n ≤ i + n := Nat.le_add_left n i
+  have hx : j < i + n := Nat.lt_of_lt_of_le h2 hy
+  simp [Nat.sub_lt_left_of_lt_add h1 hx]
