Regex/Syntax/Translate.lean
@@ -4,6 +4,8 @@ import Regex.Syntax.Ast.Visitor
 import Regex.Syntax.Hir
 import Regex.Utils
 import Regex.Unicode
+import Regex.Data.Char.Basic
+
 import UnicodeBasic
 
 /-!
@@ -84,9 +86,9 @@ private def ast_literal_to_scalar (lit: Ast.Literal) : Except String Char :=
 private def push_char (c : Char) (stack : Array HirFrame) : Array HirFrame :=
   stack.push (HirFrame.Literal c)
 
-private def unicode_fold_and_negate (cls : ClassUnicode) (flags : Flags) (negate : Bool)
+private def unicode_fold_and_negate (ranges : Array ClassUnicodeRange) (flags : Flags) (negate : Bool)
     : ClassUnicode :=
-  let cls := ClassUnicode.canonicalize cls
+  let cls : ClassUnicode := ⟨Interval.canonicalize ranges⟩
   let cls := if flags.is_case_insensitive then ClassUnicode.case_fold cls else cls
   if negate then ClassUnicode.negate cls else cls
 
@@ -136,47 +138,50 @@ private def hir_unicode_class (cls : Ast.ClassUnicode) (flags : Flags)
     match cls.kind with
     | .OneLetter c =>
         let range ← range_of_category c.toString
-        Except.ok (unicode_fold_and_negate ⟨⟨range⟩⟩ flags cls.negated)
+        Except.ok (unicode_fold_and_negate range flags cls.negated)
     | .Named s =>
       let range ← range_of_category s
-      Except.ok (unicode_fold_and_negate ⟨⟨range⟩⟩ flags cls.negated)
+      Except.ok (unicode_fold_and_negate range flags cls.negated)
     | .NamedValue _ n s =>
       let range ← range_of_named_property n s
-      Except.ok (unicode_fold_and_negate ⟨⟨range⟩⟩ flags cls.negated)
+      Except.ok (unicode_fold_and_negate range flags cls.negated)
 
 private def hir_perl_unicode_class (cls : Ast.ClassPerl) (flags : Flags)
     : Except String ClassUnicode := do
   match cls.kind with
   | .Digit =>
     let range : Array ClassUnicodeRange ← range_of_general_category Unicode.GeneralCategory.Nd
-    Except.ok (unicode_fold_and_negate ⟨⟨range⟩⟩ flags cls.negated)
+    Except.ok (unicode_fold_and_negate range flags cls.negated)
   | .Space =>
     let range : Array ClassUnicodeRange ← range_of_property "White_Space"
-    Except.ok (unicode_fold_and_negate ⟨⟨range⟩⟩ flags cls.negated)
+    Except.ok (unicode_fold_and_negate range flags cls.negated)
   | .Word =>
     let range : Array ClassUnicodeRange ← range_of_property "Word"
-    Except.ok (unicode_fold_and_negate ⟨⟨range⟩⟩ flags cls.negated)
+    Except.ok (unicode_fold_and_negate range flags cls.negated)
 
 private def hir_ascii_unicode_class (cls: Ast.ClassAscii) (flags : Flags)
     : Except String ClassUnicode := do
   let range : Array ClassUnicodeRange :=
     match cls.kind with
-    | .Alnum => #[⟨'0','9'⟩, ⟨'A','Z'⟩, ⟨'a','z'⟩]
-    | .Alpha => #[⟨'A','Z'⟩, ⟨'a','z'⟩]
-    | .Ascii => #[⟨'\x00', '\x7F'⟩]
-    | .Blank => #[⟨'\t','\t'⟩, ⟨' ',' '⟩]
-    | .Cntrl => #[⟨'\x00', '\x1F'⟩, ⟨'\x7F', '\x7F'⟩]
-    | .Digit => #[⟨'0','9'⟩]
-    | .Graph => #[⟨'!','~'⟩]
-    | .Lower => #[⟨'a','z'⟩]
-    | .Print => #[⟨' ','~'⟩]
-    | .Punct => #[⟨'!','/'⟩, ⟨':','@'⟩, ⟨'[','`'⟩, ⟨'{','~'⟩]
-    | .Space => #[⟨'\t','\t'⟩, ⟨'¬','¬'⟩, ⟨'\x0B', '\x0C'⟩, ⟨'\r','\r'⟩, ⟨' ',' '⟩]
-    | .Upper => #[⟨'A','Z'⟩]
-    | .Word => #[⟨'0','9'⟩, ⟨'A','Z'⟩, ⟨'_','_'⟩, ⟨'a','z'⟩]
-    | .Xdigit => #[⟨'0','9'⟩, ⟨'A','F'⟩, ⟨'a','f'⟩]
+    | .Alnum => #[⟨'0','9', by simp_arith⟩, ⟨'A','Z', by simp_arith⟩, ⟨'a','z', by simp_arith⟩]
+    | .Alpha => #[⟨'A','Z', by simp_arith⟩, ⟨'a','z', by simp_arith⟩]
+    | .Ascii => #[⟨'\x00', '\x7F', by simp_arith⟩]
+    | .Blank => #[⟨'\t','\t', by simp_arith⟩, ⟨' ',' ', by simp_arith⟩]
+    | .Cntrl => #[⟨'\x00', '\x1F', by simp_arith⟩, ⟨'\x7F', '\x7F', by simp_arith⟩]
+    | .Digit => #[⟨'0','9', by simp_arith⟩]
+    | .Graph => #[⟨'!','~', by simp_arith⟩]
+    | .Lower => #[⟨'a','z', by simp_arith⟩]
+    | .Print => #[⟨' ','~', by simp_arith⟩]
+    | .Punct => #[⟨'!','/', by simp_arith⟩, ⟨':','@', by simp_arith⟩, ⟨'[','`', by simp_arith⟩,
+        ⟨'{','~', by simp_arith⟩]
+    | .Space => #[⟨'\t','\t', by simp_arith⟩, ⟨'¬','¬', by simp_arith⟩,
+        ⟨'\x0B', '\x0C', by simp_arith⟩, ⟨'\r','\r', by simp_arith⟩, ⟨' ',' ', by simp_arith⟩]
+    | .Upper => #[⟨'A','Z', by simp_arith⟩]
+    | .Word => #[⟨'0','9', by simp_arith⟩, ⟨'A','Z', by simp_arith⟩, ⟨'_','_', by simp_arith⟩,
+        ⟨'a','z', by simp_arith⟩]
+    | .Xdigit => #[⟨'0','9', by simp_arith⟩, ⟨'A','F', by simp_arith⟩, ⟨'a','f', by simp_arith⟩]
 
-  Except.ok (unicode_fold_and_negate ⟨⟨range⟩⟩ flags cls.negated)
+  Except.ok (unicode_fold_and_negate range flags cls.negated)
 
 private def hir_assertion (ast : Ast.Assertion) (flags : Syntax.Flags) : Hir :=
   let multi_line := flags.is_multi_line
@@ -299,7 +304,7 @@ def visit_post (ast: Ast) : StateT Translator (Except String) PUnit := do
     let c ← ast_literal_to_scalar lit
     if t.flags.is_case_insensitive
     then
-      let ranges : IntervalSet Char := ⟨Unicode.case_fold_char c⟩
+      let ranges : IntervalSet Char := Interval.canonicalize (Unicode.case_fold_char c)
       let cls : ClassUnicode := ClassUnicode.canonicalize ⟨ranges⟩
       let kind := (HirKind.Class (Class.Unicode cls))
       let expr := Hir.mk kind (Hir.toProperties kind)
@@ -313,7 +318,7 @@ def visit_post (ast: Ast) : StateT Translator (Except String) PUnit := do
     match t.stack.pop? with
     | some (frame, stack) =>
       let cls ← frame.unwrap_class_unicode
-      let cls := unicode_fold_and_negate cls t.flags ast.negate
+      let cls := unicode_fold_and_negate cls.set.ranges t.flags ast.negate
       let kind := (HirKind.Class (Class.Unicode cls))
       let expr := Hir.mk kind (Hir.toProperties kind)
       set {t with stack := stack.push (HirFrame.Expr expr)}
@@ -382,16 +387,16 @@ def visit_class_set_item_post (ast : ClassSetItem)
     match t.stack.pop? with
     | some (frame, stack) =>
       let cls ← frame.unwrap_class_unicode
-      let ranges := cls.set.ranges.push ⟨lit.c, lit.c⟩
-      let cls := ⟨ClassUnicode.set ⟨⟨ranges⟩⟩⟩
+      let ranges := cls.set.ranges.push ⟨lit.c, lit.c, by simp [Char.eq_le _]⟩
+      let cls := ⟨ClassUnicode.set ⟨Interval.canonicalize ranges⟩⟩
       set {t with stack := stack.push (HirFrame.ClassUnicode cls)}
     | none => Except.error "visit_class_set_item_post .Literal in stack expected"
   | .Range range =>
     match t.stack.pop? with
     | some (frame, stack) =>
       let cls ← frame.unwrap_class_unicode
-      let ranges := cls.set.ranges.push ⟨range.start.c, range.end.c⟩
-      let cls := ⟨ClassUnicode.set ⟨⟨ranges⟩⟩⟩
+      let ranges := cls.set.ranges.push ⟨range.start.c, range.end.c, range.isLe⟩
+      let cls := ⟨ClassUnicode.set ⟨Interval.canonicalize ranges⟩⟩
       set {t with stack := stack.push (HirFrame.ClassUnicode cls)}
     | none => Except.error "visit_class_set_item_post .Range in stack expected"
   | .Ascii asciicls =>
@@ -424,7 +429,7 @@ def visit_class_set_item_post (ast : ClassSetItem)
       match stack.pop? with
       | some (cls2, stack) =>
         let cls1 ← cls1.unwrap_class_unicode
-        let cls1 := unicode_fold_and_negate cls1 t.flags ast.negate
+        let cls1 := unicode_fold_and_negate cls1.set.ranges t.flags ast.negate
         let cls2 ← cls2.unwrap_class_unicode
         set {t with stack :=
           stack.push (HirFrame.ClassUnicode (ClassUnicode.union cls1 cls2))}
@@ -456,9 +461,9 @@ def visit_class_set_binary_op_post (op: ClassSetBinaryOp)
       match stack.pop? with
       | some (cls, stack) =>
         let lhs ← lhs.unwrap_class_unicode
-        let lhs := unicode_fold_and_negate lhs t.flags false
+        let lhs := unicode_fold_and_negate lhs.set.ranges t.flags false
         let rhs ← rhs.unwrap_class_unicode
-        let rhs := unicode_fold_and_negate rhs t.flags false
+        let rhs := unicode_fold_and_negate rhs.set.ranges t.flags false
         let cls ← cls.unwrap_class_unicode
         let clsOfKind :=
           match op.kind with
