Regex/Unicode/Utils.lean
@@ -23,6 +23,11 @@ def toRange (val : UInt32 × Option UInt32) : Range Char :=
   let (u1, u2) := val
   let u2 := match u2 with | some u2 => u2 | none => u1
   if h1 : UInt32.isValidChar u1 then
-    if h2 : UInt32.isValidChar u2 then ⟨⟨u1, h1⟩, ⟨u2, h2⟩⟩
-    else ⟨default, default⟩
-  else ⟨default, default⟩
+    if h2 : UInt32.isValidChar u2
+      then
+        let c1 : Char := ⟨u1, h1⟩
+        let c2 : Char := ⟨u2, h2⟩
+        if h3 : c1 ≤ c2 then ⟨c1, c2, h3⟩
+        else ⟨default, default, by simp_arith⟩
+    else ⟨default, default, by simp_arith⟩
+  else ⟨default, default, by simp_arith⟩
